IL/Sim.v
@@ -1,5 +1,5 @@
 Require Import List.
-Require Export Util Var Val Exp Env Map CSet AutoIndTac IL.
+Require Export Util Var Val Exp Env Map CSet AutoIndTac IL AllInRel.
 
 Set Implicit Arguments.
 Unset Printing Records.
@@ -290,60 +290,7 @@ eapply simeq_refl.
 eapply simeq_sym. eapply obseq_simeq; eauto.
 eapply simeq_trans; eapply obseq_simeq; eauto.
 Qed.
-
-
-(** * Contextual Equivalence *)
-
-Inductive stmtCtx : Type :=
-| ctxExp    (x : var) (e: exp) (C : stmtCtx) : stmtCtx
-| ctxIfS     (e : exp) (C : stmtCtx) (t : stmt) : stmtCtx
-| ctxIfT     (e : exp) (s : stmt) (C : stmtCtx) : stmtCtx
-(* block f Z : rt = s in b  *)
-| ctxLetS    (Z:params) (C : stmtCtx) (t : stmt) : stmtCtx 
-| ctxLetT    (Z:params) (s : stmt) (C : stmtCtx) : stmtCtx
-| ctxHole.
-
-Fixpoint fill (ctx:stmtCtx) (s':stmt) : stmt :=
-  match ctx with
-    | ctxExp x e ctx => stmtExp x e (fill ctx s')
-    | ctxIfS e ctx t => stmtIf e (fill ctx s') t
-    | ctxIfT e s ctx => stmtIf e s (fill ctx s')
-    | ctxLetS Z ctx t => stmtLet Z (fill ctx s') t 
-    | ctxLetT Z s ctx => stmtLet Z s (fill ctx s')
-    | ctxHole => s'
-  end.
-
-Fixpoint fillC (ctx:stmtCtx) (s':stmtCtx) : stmtCtx :=
-  match ctx with
-    | ctxExp x e ctx => ctxExp x e (fillC ctx s')
-    | ctxIfS e ctx t => ctxIfS e (fillC ctx s') t
-    | ctxIfT e s ctx => ctxIfT e s (fillC ctx s')
-    | ctxLetS Z ctx t => ctxLetS Z (fillC ctx s') t 
-    | ctxLetT Z s ctx => ctxLetT Z s (fillC ctx s')
-    | ctxHole => s'
-  end.
-
-Definition ctxeq (s s':stmt) :=
-  forall ctx E, cobehave (nil:list F.block, E, (fill ctx s)) (nil:list F.block, E, (fill ctx s')).
  
-
-(*
-Lemma foo s s' E E' Z L t
-: simeq s s'
-  -> paco0 sim ((F.blockI E' Z s :: L)%list, E, t)
-         ((F.blockI E' Z s' :: L)%list, E, t).
-Proof.  
-  revert s s' E E' Z L t. pcofix foo. intros.
-  destruct t. 
-  exfalso; clear_all.
-  exfalso; clear_all.
-  + destruct l. destruct n.
-    econstructor. eapply plusO. econstructor; eauto using get. exfalso; clear_all.
-    eapply plusO. econstructor; eauto using get. exfalso; clear_all. simpl.
-    refine (sim_trans (foo s s' (updE E' E Z Y) E' Z L s H) _). Guarded.
-Qed.  
-*)
-
 Lemma subst_lemma_div L' s s' E E' Z L t
 : obseq s s'
   -> diverges step ((L' ++ F.blockI E' Z s :: L)%list, E, t)
@@ -364,7 +311,8 @@ Proof.
         simpl. rewrite H5. rewrite drop_length_eq.
         eapply (subst_lemma_div nil); eauto. simpl. 
         rewrite H5 in H2. rewrite drop_length_eq in H2.
-        edestruct (H (F.blockI E' Z s :: L) (E'[Z <-- vl])). erewrite <- H3. eauto.
+        edestruct (H (F.blockI E' Z s :: L) (E'[Z <-- List.map Some vl])).
+        erewrite <- H3. eauto.
       * econstructor. econstructor; eauto.
         rewrite cons_app. rewrite app_assoc. 
         eapply get_app_right; eauto. simpl.
@@ -415,11 +363,11 @@ Proof.
     assert (drop (length L') (L' ++ F.blockI E' Z s :: L)
             = (F.blockI E' Z s :: L) % list).
     eapply drop_length_eq.
-    pose proof (IHterminatesWith nil _ _ (E'[Z <-- vl]) E' Z L s H1 eq_refl).
+    pose proof (IHterminatesWith nil _ _ (E'[Z <-- List.map Some vl]) E' Z L s H1 eq_refl).
     rewrite H4 in H3. rewrite H2 in H3.
     simpl in *. specialize (H3 eq_refl).
     hnf in H1.
-    pose proof (H1 (drop (labN l) (L' ++ F.blockI E' Z s' :: L)) (E'[Z <-- vl])).
+    pose proof (H1 (drop (labN l) (L' ++ F.blockI E' Z s' :: L)) (E'[Z <-- List.map Some vl])).
     eapply H5; rewrite H4. rewrite drop_length_eq. eauto.
     eapply trmWithStep. 
     eapply F.stepGoto with (blk:=blk); eauto.
@@ -443,116 +391,16 @@ Proof.
   eapply (subst_lemma_trm nil); eauto.
   eapply (subst_lemma_trm nil); eauto. symmetry; eauto.
 Qed.
-  
 
-Lemma simeq_contextual s s' ctx
-  : simeq s s' -> simeq (fill ctx s) (fill ctx s').
-Proof.
-  intros. general induction ctx; simpl; hnf; intros.
-  + destruct (step_dec (L, E, stmtExp x e (fill ctx s))). destruct H0.
-    inv H0.
-    eapply simS; simpl; eauto using plus, F.step. eapply IHctx; eauto.
-    eapply simE; try eapply star_refl. eauto. eauto.
-    simpl. destruct 1. inv H1. eapply H0. 
-    econstructor. econstructor; eauto.
-  + case_eq (exp_eval E e); intros.
-    case_eq (val2bool v); intros.
-    eapply simS.
-    econstructor. econstructor; eauto.
-    econstructor; econstructor; eauto. eapply IHctx; eauto.
-    eapply simS.
-    econstructor. eapply F.stepIfF; eauto.
-    econstructor; eapply F.stepIfF; eauto.
-    eapply sim_refl.
-    eapply simE; try eapply star_refl; eauto; stuck.
-  + case_eq (exp_eval E e); intros.
-    case_eq (val2bool v); intros.
-    eapply simS; auto.
-    econstructor. econstructor; eauto.
-    econstructor; econstructor; eauto.
-    eapply sim_refl.
-    eapply simS.
-    econstructor. eapply F.stepIfF; eauto.
-    econstructor; eapply F.stepIfF; eauto. eapply IHctx; eauto.
-    eapply simE; try eapply star_refl; eauto; stuck.
-  + eapply simS.
-    eapply plusO. econstructor.
-    eapply plusO. econstructor.
-    specialize (IHctx _ _ H).
-    eapply obseq_simeq in IHctx.
-    pose proof (subst_lemma E E Z L t IHctx). eauto.
-  + econstructor.
-    econstructor; econstructor.
-    econstructor; econstructor.
-    eapply IHctx; eauto.
-  + eapply H; eauto using lsim_refl.
-Qed. 
-
-Lemma fill_fillC C C' s
-  :  fill (fillC C C') s = fill C (fill C' s).
-Proof.
-  general induction C; simpl; f_equal; eauto.
-Qed.
-
-
+(*
 Inductive approx : F.block -> F.block -> Prop :=
  | approxI E E' Z s
    : agree_on (freeVars s \ of_list Z) E E'
      -> approx (F.blockI E Z s) (F.blockI E' Z s).
 
-Require Import AllInRel.
 
-
-Lemma ctx_constr_E E' G G' 
-  : exists C, forall E, exists EC, forall (L:list F.block) s, star step (L, E, fill C s) (L, EC, s) 
-                    /\ agree_on G EC E'
-                    /\ agree_on (G'\G) EC E.
-Proof.
-  pattern G. eapply set_induction.
-  intros. eexists ctxHole. intros. eexists E. 
-  split. eapply star_refl. eapply empty_is_empty_1 in H.  rewrite H.
-  split. hnf; intros; cset_tac; intuition. eapply agree_on_refl.
-  intros. edestruct H as [C' ?].
-  eexists (fillC C' (ctxExp x (Con (E' x)) ctxHole)).
-  intros. specialize (H2 E). destruct H2 as[EC' ?].
-  eexists (EC'[x<-E' x]). intros. rewrite fill_fillC.
-  split. simpl. eapply star_right. eapply H2.
-  econstructor. simpl; eauto.
-  split. hnf; intros. lud; eqs. rewrite e. eauto.
-  eapply H2; eauto. edestruct H1. specialize (H6 H3). destruct H6; intuition.
-  eapply agree_on_update_dead. cset_tac; intuition. eapply H5. eapply H1; intuition.
-  eapply agree_on_incl; eauto. eapply H2; eauto. eapply Add_Equal in H1. 
-  rewrite H1. cset_tac; intuition.
-Qed.
-
-Lemma ctx_constr (L:list F.block) E G L'
-  : exists C E' LC, forall s, star step (L, E, fill C s) ((LC++L)%list, E', s) 
-                    /\ agree_on G E E' 
-                    /\ PIR2 approx LC L'.
-Proof.
-  intros. general induction L'.
-  + eexists ctxHole, E, nil; simpl. 
-    repeat split. eapply star_refl. constructor.
-  + destruct a.  
-    edestruct (ctx_constr_E block_E (freeVars block_s) ∅) as [CE].
-    edestruct (ctx_constr_E E G) as [CE2]. instantiate (1:=∅) in H0.
-    edestruct (IHL' L E G) as [CR [ER [LC' ]]].
-    specialize (H ER). destruct H as [CEE ?].
-    specialize (H0 CEE). destruct H0 as [CEE2 ?].
-    eexists (fillC CR (fillC CE (ctxLetT block_Z block_s CE2))).
-    eexists CEE2, (F.blockI CEE block_Z block_s:: LC'). 
-    intros. rewrite fill_fillC.
-    specialize (H (LC'++L)%list (fill (ctxLetT block_Z block_s CE2) s)).
-    split. eapply star_trans. eapply H1.
-    rewrite fill_fillC. eapply star_trans.
-    eapply H. simpl. eapply S_star. econstructor.
-    dcr. edestruct H0. eapply H.
-    split. eapply agree_on_sym. eapply H0; eauto. 
-    econstructor. econstructor. eapply agree_on_incl. eapply H. 
-    eapply incl_minus. eapply H1; eauto.
-Qed.
   
-Lemma sim_freeVars (L L':list F.block) (E E':env var) s
+Lemma sim_freeVars (L L':list F.block) (E E':onv var) s
 :  agree_on (freeVars s) E E'
    -> PIR2 approx L L'
    -> sim (L, E, s) (L', E', s).
@@ -655,7 +503,7 @@ Proof.
   pose proof (@sim_freeVars L L' E E' s' H3 H1).
   eapply sim_sym in H4.
   eapply (sim_trans H4 (sim_trans H H5)).
-Qed.
+Qed.*)
 
 Lemma sim_reduction_closed {S} `{StateType S} {S'} `{StateType S'} 
       (σ1 σ1':S) (σ2 σ2':S')
@@ -688,32 +536,6 @@ Proof.
   eapply terminatesWith_star; eauto. eapply H4. eapply terminatesWith_star_2; eauto.
   eapply terminatesWith_star; eauto. eapply H4. eapply terminatesWith_star_2; eauto.
 Qed.
-
-Lemma ctxeq_simeq s s':
-  ctxeq s s' <-> simeq s s'.
-Proof.
-  split; intros. 
-  hnf; intros. edestruct (ctx_constr (nil:list F.block) E (freeVars s ∪ freeVars s')) as [C [E' [LC ?]]].
-  specialize (H C E); simpl in *. 
-  eapply sim_cobehave in H; eauto.
-  pose proof (H0 s). specialize (H0 s'); dcr.
-  pose proof (sim_reduction_closed H H2 H1).
-  repeat rewrite app_nil_r in H0.
-  eapply sim_coincidence; eauto.
-  symmetry; eauto.
-  hnf; intros. 
-  eapply sim_cobehave. eapply simeq_contextual; eauto.
-Qed.
-
-Instance ctxeq_equivalence : Equivalence ctxeq.
-Proof.
-  hnf; intros. constructor.
-  hnf; intros. eapply ctxeq_simeq; reflexivity.
-  hnf; intros. eapply ctxeq_simeq; eapply ctxeq_simeq in H; symmetry; eauto.
-  hnf; intros. eapply ctxeq_simeq. eapply ctxeq_simeq in H; eapply ctxeq_simeq in H0;
-                                   transitivity y; eauto.
-Qed.
-
 
 Ltac single_step :=
   match goal with
@@ -812,10 +634,10 @@ Proof.
       reflexivity. simpl. rewrite H7. rewrite drop_length_eq.
       eapply (subst_lemma_div_L nil); eauto. simpl. 
       rewrite H7 in H4. rewrite drop_length_eq in H4.
-      specialize (H vl).
+      specialize (H (List.map Some vl)).
       pose proof (@sim_codiverge F.state _ F.state _).
-      eapply H5; eauto. eapply H. symmetry in len.
-      erewrite <- omap_length; eauto. congruence.
+      eapply H5; eauto. eapply H. symmetry in len. 
+      exploit omap_length; eauto. rewrite map_length. congruence. congruence.
       eapply simL_refl.
     - edestruct (AIR4_length H1); dcr.
       destruct (AIR4_nth' H1 H6) as [? [? [?]]]; dcr.
@@ -828,7 +650,8 @@ Proof.
       rewrite drop_length_gr in H4; eauto.
       pose proof (@sim_codiverge F.state _ F.state _).
       eapply H6. eapply H14. symmetry in len. 
-      erewrite <- omap_length; try eapply def. congruence. congruence.
+      exploit omap_length; try eapply def. rewrite map_length.
+      congruence. congruence.
       eauto. 
   + econstructor. econstructor.
     rewrite cons_app. rewrite app_assoc.
@@ -885,9 +708,10 @@ Proof.
         simpl.
         rewrite H4 in *. erewrite drop_length_eq in *. 
         simpl in *. rewrite H4. erewrite drop_length_eq. 
-        refine (sim_coterminatesWith (LEQ vl _ _ 
+        refine (sim_coterminatesWith (LEQ (List.map Some vl) _ _ 
                                                _ _ (simL_refl _)) _).
-        erewrite <- omap_length; try eapply def. congruence. congruence.
+        exploit omap_length; try eapply def. rewrite map_length. 
+        congruence. congruence.
         eapply (IHterminatesWith nil); eauto. 
       * dcr.
         edestruct AIR4_length; try eassumption; dcr.
@@ -902,7 +726,8 @@ Proof.
         rewrite drop_length_gr in H0; eauto.
         simpl. 
         refine (sim_coterminatesWith (H10 _ _ _) _). 
-        erewrite <- omap_length; try eapply def. congruence. congruence.
+        exploit omap_length; try eapply def. rewrite map_length.
+        congruence. congruence.
         eapply H0.
     - eapply trmWithStep. econstructor; eauto.
       rewrite cons_app. rewrite app_assoc.
@@ -959,7 +784,8 @@ Proof.
     - edestruct AIR4_nth' as [? [? [? ]]]; dcr; try eassumption.
       repeat get_functional; subst. inv H6.
       one_step; simpl in *; eauto. congruence. simpl.
-      eapply H11; eauto. erewrite <- omap_length; try eapply H0; eauto.
+      eapply H11; eauto. exploit omap_length; try eapply H0; eauto.
+      rewrite map_length; congruence.
     - no_step.
     - edestruct AIR4_nth' as [? [? [? ]]]; dcr; try eassumption.
       repeat get_functional; subst. inv H5.
